finished a first version of Ordered Terms

theories/Ordered/OrderedType.v
@@ -132,6 +132,10 @@ Program Definition OTType : OType :=
 *)
 
 
+(***
+ *** The Ordered Type for Functions
+ ***)
+
 (* The type of continuous, i.e. Proper, functions between ordered types *)
 Record Pfun (A:OType) (B: OType) :=
   {
@@ -158,6 +162,46 @@ Next Obligation.
     - apply (Rfg a1 a1). reflexivity.
     - apply Rgh; assumption. }
 Qed.
+
+(* Curry a Pfun *)
+Program Definition pfun_curry {A B C} (pfun : Pfun (OTpair A B) C)
+  : Pfun A (OTarrow B C) :=
+  {| pfun_app :=
+       fun a =>
+         {| pfun_app := fun b => pfun_app pfun (a,b);
+            pfun_Proper := _ |};
+     pfun_Proper := _ |}.
+Next Obligation.
+Proof.
+  intros b1 b2 Rb. apply pfun_Proper.
+  split; [ reflexivity | assumption ].
+Qed.
+Next Obligation.
+Proof.
+  intros a1 a2 Ra b1 b2 Rb; simpl.
+  apply pfun_Proper; split; assumption.
+Qed.
+
+(* Uncrry a Pfun *)
+Program Definition pfun_uncurry {A B C} (pfun : Pfun A (OTarrow B C))
+  : Pfun (OTpair A B) C :=
+  {| pfun_app :=
+       fun ab => pfun_app (pfun_app pfun (fst ab)) (snd ab);
+     pfun_Proper := _ |}.
+Next Obligation.
+Proof.
+  intros ab1 ab2 Rab. destruct Rab as [ Ra Rb ].
+  exact (pfun_Proper pfun (fst ab1) (fst ab2) Ra (snd ab1) (snd ab2) Rb).
+Qed.
+
+(* Currying and uncurrying of pfuns form an adjunction *)
+(* FIXME HERE: figure out the simplest way of stating this adjunction *)
+
+
+(* OTarrow is right adjoint to OTpair, meaning that (OTarrow (OTpair A B) C) is
+isomorphic to (OTarrow A (OTarrow B C)). The following is the first part of this
+isomorphism, mapping left-to-right. *)
+
 
 (* FIXME: could also do a forall type, but need the second type argument, B, to
 itself be proper, i.e., to be an element of OTArrow A OType. Would also need a
@@ -198,6 +242,29 @@ Instance OTCtxExtends_cons_right ctx1 ctx2
          {ext:OTCtxExtends ctx1 ctx2} {B} : OTCtxExtends ctx1 (OTpair ctx2 B) :=
   ContextExtends_cons_right _ context_extends.
 
+(* Context extension induces a mapping from the bigger to the smaller context *)
+Fixpoint unextend_context {ctx1 ctx2} (ext: ContextExtends ctx1 ctx2) :
+  ot_Type ctx2 -> ot_Type ctx1 :=
+  match ext in ContextExtends ctx1 ctx2 return ot_Type ctx2 -> ot_Type ctx1 with
+  | ContextExtends_refl ctx => fun celem => celem
+  | ContextExtends_cons_both A ext' =>
+    fun celem =>
+      (unextend_context ext' (fst celem), snd celem)
+  | ContextExtends_cons_right A ext' =>
+    fun celem =>
+      unextend_context ext' (fst celem)
+  end.
+
+(* unextend_context preserves ordering *)
+Instance unextend_context_Proper {ctx1 ctx2} ext :
+  Proper (ot_R ctx2 ==> ot_R ctx1) (unextend_context ext).
+Proof.
+  induction ext; simpl; intros celem1 celem2 R12.
+  { assumption. }
+  { destruct R12; split; [ apply IHext | ]; assumption. }
+  { destruct R12. apply IHext. assumption. }
+Qed.
+
 
 (***
  *** Ordered Terms in Context
@@ -207,441 +274,55 @@ Instance OTCtxExtends_cons_right ctx1 ctx2
 Inductive OTermInCtx ctx A : Type :=
   | mkOTermInCtx (pfun: Pfun ctx A).
 
+Arguments mkOTermInCtx {ctx A} pfun.
+
+(* Helper to eliminate an OTermInCtx *)
 Definition elimOTermInCtx {ctx A} (oterm: OTermInCtx ctx A) : Pfun ctx A :=
   let (pfun) := oterm in pfun.
 
-
-FIXME HERE NOW: apply a OTCtxtExtends proof to a variable, and then do
-proper_fun!
-
-
-(* An ordered type context is a list of ordered types *)
-Definition OTContext := list OType.
-
-(* An element of an ordered type context is an element of each ordered type *)
-Fixpoint ctx_elem (ctx:OTContext) : Type :=
-  match ctx with
-  | [] => unit
-  | A::ctx' => (ot_Type A) * (ctx_elem ctx')
-  end.
-
-(* The ordering on ordered type context elements is the pointwise orderings of
-all the ordered types in the context *)
-Fixpoint ctx_elem_lt (ctx:OTContext) : relation (ctx_elem ctx) :=
-  match ctx with
-  | [] => fun _ _ => True
-  | A::ctx' => fun e1 e2 =>
-                 validR (ot_R A) (fst e1) (fst e2) /\
-                 ctx_elem_lt ctx' (snd e1) (snd e2)
-  end.
-
-(* Consing two ordered objects to two ordered context elements yields two
-ordered context elements *)
-Lemma ctx_elem_lt_cons ctx A celem1 celem2 a1 a2
-      (pf_ctx: validR (ctx_elem_lt ctx) celem1 celem2)
-      (pf_A : validR (ot_R A) a1 a2) :
-  validR (ctx_elem_lt (A::ctx)) (a1,celem1) (a2,celem2).
-  unfold ctx_elem_lt; fold ctx_elem_lt.
-  destruct pf_ctx; destruct pf_A.
-  repeat split; assumption.
-Qed.
-
-(* The ordered type of context elements *)
-Program Definition OTCtxElem (ctx:OTContext) : OType :=
-  {|
-    ot_Type := ctx_elem ctx;
-    ot_R := ctx_elem_lt ctx;
-  |}.
-Next Obligation.
-  induction ctx; constructor.
-  { intros; assumption. }
-  { repeat (intro foo; destruct foo). split.
-    - destruct H; destruct H3; destruct H5; destruct H7.
-      split; try assumption.
-      apply (@semitransitivity _ _ (ot_PreOrder a) _ (fst (o0, c0)));
-        try assumption.
-    - apply (semitransitivity _ (snd (o0, c0))); assumption.
-  }
-Qed.
-
-(* The ordered type of objects-in-context *)
-Definition OTInCtx (ctx:OTContext) (A:OType) : OType :=
-  OTArrow (OTCtxElem ctx) A.
-
-
-(***
- *** Context Extensions
- ***)
-
-(* Captures that one context extends another. Note that we put this in Type
-instead of Prop so we can induct on it. *)
-Inductive ContextExtends : OTContext -> OTContext -> Type :=
-| ContextExtends_nil : ContextExtends [] []
-| ContextExtends_cons_both {ctx1 ctx2} A :
-    ContextExtends ctx1 ctx2 -> ContextExtends (A::ctx1) (A::ctx2)
-| ContextExtends_cons_right {ctx1 ctx2} A :
-    ContextExtends ctx1 ctx2 -> ContextExtends ctx1 (A::ctx2)
-.
-
-(* Context extension is reflexive *)
-Definition ContextExtends_reflexive ctx : ContextExtends ctx ctx.
-  induction ctx; constructor; assumption.
-Defined.
-
-(* Context extension as a type class *)
-Class OTCtxExtends ctx1 ctx2 : Type :=
-  context_extends : ContextExtends ctx1 ctx2.
-
-Arguments context_extends {_ _ _}.
-
-(* The rules for context extension, as type class instances *)
-Instance OTCtxExtends_refl ctx : OTCtxExtends ctx ctx :=
-  ContextExtends_reflexive _.
-
-Instance OTCtxExtends_cons_both ctx1 ctx2
-         {ext:OTCtxExtends ctx1 ctx2} {B} : OTCtxExtends (B::ctx1) (B::ctx2) :=
-  ContextExtends_cons_both _ context_extends.
-
-Instance OTCtxExtends_cons_right ctx1 ctx2
-         {ext:OTCtxExtends ctx1 ctx2} {B} : OTCtxExtends ctx1 (B::ctx2) :=
-  ContextExtends_cons_right _ context_extends.
-
-
-(* "Forget" elements of an extended context to get an un-extended context *)
-Fixpoint context_forget {ctx1 ctx2} (ext: OTCtxExtends ctx1 ctx2) :
-  ctx_elem ctx2 -> ctx_elem ctx1 :=
-  match ext in ContextExtends ctx1 ctx2
-        return ctx_elem ctx2 -> ctx_elem ctx1 with
-    | ContextExtends_nil => fun celem => celem
-    | ContextExtends_cons_both A ext' =>
-      fun celem =>
-        let (a,celem') := celem in
-        (a, context_forget ext' celem')
-    | ContextExtends_cons_right A ext' =>
-      fun celem =>
-        let (a,celem') := celem in
-        context_forget ext' celem'
-  end.
-
-(* Forgetting preserves context element ordering *)
-Lemma context_forget_preserves {ctx1 ctx2} ext celem2_1 celem2_2 :
-  ctx_elem_lt ctx2 celem2_1 celem2_2 ->
-  ctx_elem_lt ctx1 (context_forget ext celem2_1) (context_forget ext celem2_2).
-  revert celem2_1 celem2_2; induction ext; intros.
-  { unfold context_forget; assumption. }
-  { unfold context_forget; fold (context_forget ext).
-    destruct celem2_1; destruct celem2_2. destruct H; destruct H.
-    repeat constructor; unfold fst in * |- *; try assumption.
-    apply IHext; assumption. }
-  { unfold context_forget; fold (context_forget ext).
-    destruct celem2_1; destruct celem2_2. destruct H; destruct H.
-    apply IHext; assumption. }
-Qed.
-
-(* Forgetting thus preserves valid context element ordering *)
-Lemma context_forget_preserves_validR {ctx1 ctx2} ext celem2_1 celem2_2 :
-  validR (ctx_elem_lt ctx2) celem2_1 celem2_2 ->
-  validR (ctx_elem_lt ctx1)
-         (context_forget ext celem2_1) (context_forget ext celem2_2).
-  intro pf; destruct pf.
-  repeat constructor; apply context_forget_preserves; assumption.
-Qed.
-
-
-(***
- *** Pairs of Related Elements
- ***)
-
-(* Pairs of terms-in-context that are valid and related to each other *)
-Inductive OTPairInCtx ctx A : Type :=
-  mkOTPairInCtx (x1: ctx_elem ctx -> ot_Type A)
-                (x2: ctx_elem ctx -> ot_Type A)
-                (pf: validR (ot_R (OTInCtx ctx A)) x1 x2) :
-    OTPairInCtx ctx A.
-
-(* Weakening the context of an OTPairInCtx *)
+(* Weakening the context of an OTermInCtx *)
 Program Definition weaken_context {ctx1 ctx2} {ext: OTCtxExtends ctx1 ctx2}
-           {A} (p: OTPairInCtx ctx1 A) : OTPairInCtx ctx2 A :=
+           {A} (p: OTermInCtx ctx1 A) : OTermInCtx ctx2 A :=
   match p with
-    | mkOTPairInCtx _ _ x1 x2 pf =>
-      mkOTPairInCtx _ _ (fun celem1 => x1 (context_forget ext celem1))
-                    (fun celem1 => x2 (context_forget ext celem1))
-                    _
+  | mkOTermInCtx pfun =>
+    mkOTermInCtx
+      {| pfun_app := fun celem => pfun_app pfun (unextend_context ext celem);
+         pfun_Proper := _ |}
   end.
 Next Obligation.
-  destruct pf as [ pf1 pf2 pf3 ].
-  repeat constructor;
-    intros; [ apply pf1 | apply pf2 | apply pf3 ];
-    apply context_forget_preserves_validR; assumption.
+  intros celem1 celem2 R12. apply pfun_Proper.
+  apply unextend_context_Proper. assumption.
 Qed.
 
-(* Build a term-in-context for the top-most variable in the context *)
-Program Definition top_var_in_context ctx A : OTPairInCtx (A::ctx) A :=
-  mkOTPairInCtx (A::ctx) A
-           (fun ctx_elem =>
-              let (celem_A,_) := ctx_elem in celem_A)
-           (fun ctx_elem =>
-              let (celem_A,_) := ctx_elem in celem_A)
-           _.
+(* Helper to build a "variable" for the top of the context as an OTermInCtx *)
+Program Definition top_var_in_context ctx A : OTermInCtx (OTpair ctx A) A :=
+  mkOTermInCtx {| pfun_app := fun celem => snd celem;
+                  pfun_Proper := _ |}.
 Next Obligation.
-  repeat split;
-    intros x y; destruct x; destruct y; unfold fst; unfold snd;
-      intros; repeat (destruct H); repeat (destruct H0); repeat (destruct H1);
-        assumption.
-Qed.
-
-(* OTPairInCtx is a functor w.r.t. proper functions *)
-Program Definition map_OTPairInCtx {ctx A B}
-        (f: ot_Type A -> ot_Type B)
-        (proper: Proper (validR (ot_R A) ==> validR (ot_R B)) f)
-        (x: OTPairInCtx ctx A) : OTPairInCtx ctx B :=
-  let (x1,x2,pf_x) := x in
-  mkOTPairInCtx _ _ (fun celem => f (x1 celem)) (fun celem => f (x2 celem)) _.
-Next Obligation.
-  destruct pf_x as [ pfx_1 pfx_2 pfx_3 ].
-  repeat split; intros celem1 celem2 H; apply proper; repeat split;
-  first [ apply pfx_1 | apply pfx_2 | apply pfx_3 ];
-  try assumption; destruct H; repeat split; assumption.
-Qed.
-
-(* OTPairInCtx is also a bi-functor w.r.t. proper functions *)
-Program Definition map2_OTPairInCtx {ctx A B C}
-        (f: ot_Type A -> ot_Type B -> ot_Type C)
-        (proper: Proper (validR (ot_R A) ==> validR (ot_R B) ==> validR (ot_R C)) f)
-        (x: OTPairInCtx ctx A) (y: OTPairInCtx ctx B) : OTPairInCtx ctx C :=
-  let (x1,x2,pf_x) := x in
-  let (y1,y2,pf_y) := y in
-  mkOTPairInCtx _ _ (fun celem => f (x1 celem) (y1 celem))
-                (fun celem => f (x2 celem) (y2 celem)) _.
-Next Obligation.
-  destruct pf_x as [ pfx_1 pfx_2 pfx_3 ].
-  destruct pf_y as [ pfy_1 pfy_2 pfy_3 ].
-  repeat split; intros celem1 celem2 H; apply proper; repeat split;
-  first [ apply pfx_1 | apply pfy_1 | apply pfx_2 | apply pfy_2 |
-          apply pfx_3 | apply pfy_3 ];
-  try assumption; destruct H; repeat split; assumption.
-Qed.
-
-(* OTPairInCtx is also a tri-functor w.r.t. proper functions *)
-Program Definition map3_OTPairInCtx {ctx A B C D}
-        (f: ot_Type A -> ot_Type B -> ot_Type C -> ot_Type D)
-        (proper: Proper (validR (ot_R A) ==> validR (ot_R B) ==>
-                                validR (ot_R C) ==> validR (ot_R D)) f)
-        (x: OTPairInCtx ctx A) (y: OTPairInCtx ctx B) (z: OTPairInCtx ctx C)
-: OTPairInCtx ctx D :=
-  let (x1,x2,pf_x) := x in
-  let (y1,y2,pf_y) := y in
-  let (z1,z2,pf_z) := z in
-  mkOTPairInCtx _ _ (fun celem => f (x1 celem) (y1 celem) (z1 celem))
-                (fun celem => f (x2 celem) (y2 celem) (z2 celem)) _.
-Next Obligation.
-  destruct pf_x as [ pfx_1 pfx_2 pfx_3 ].
-  destruct pf_y as [ pfy_1 pfy_2 pfy_3 ].
-  destruct pf_z as [ pfz_1 pfz_2 pfz_3 ].
-  repeat split; intros celem1 celem2 H; apply proper; repeat split;
-  first [ apply pfx_1 | apply pfy_1 | apply pfz_1 |
-          apply pfx_2 | apply pfy_2 | apply pfz_2 |
-          apply pfx_3 | apply pfy_3 | apply pfz_3 ];
-  try assumption; destruct H; repeat split; assumption.
+  intros celem1 celem2 R12. destruct R12. assumption.
 Qed.
 
 
-(***
- *** Top-Level Proper Terms
- ***)
+(* Build an OTerm for a function *)
+Definition pfun_lambda {ctx} {A} {B} (f: OTermInCtx (OTpair ctx A) A ->
+                                         OTermInCtx (OTpair ctx A) B)
+  : OTermInCtx ctx (OTarrow A B) :=
+  mkOTermInCtx (pfun_curry (elimOTermInCtx (f (top_var_in_context ctx A)))).
 
-(* A "proper term" is an OTPairInCtx in the empty context *)
-Definition ProperTerm (A:OType) := OTPairInCtx [] A.
-
-(* ProperTerm is "the" way to view an OType as a Type *)
-Coercion ProperTerm : OType >-> Sortclass.
-
-(* We can coerce a ProperTerm A to an element of ot_Type A by just taking the
-first projection of the pair in the ProperTerm *)
-Definition get_proper_term {A} (p: ProperTerm A) : ot_Type A :=
-  match p with
-  | mkOTPairInCtx _ _ x1 x2 pf => x1 tt
-  end.
-
-(* Coercion coerce_proper_term : ProperTerm >-> ot_Type. *)
-
-(* Any ProperTerm is always Proper *)
-Instance ProperTerm_Proper {A} (p:ProperTerm A) :
-  Proper (ot_R A) (get_proper_term p).
-destruct p; unfold get_proper_term. destruct pf; apply H.
-repeat split.
-Qed.
-
-(* Propositions as ProperTerms *)
-Definition ProperProp := ProperTerm OTProp.
-
-(* We can view a ProperProp as a Prop *)
-Definition get_prop : ProperProp -> Prop := get_proper_term.
-Coercion get_prop : ProperProp >-> Sortclass.
-
-(* Lifting the ordering of an OType to an ordering on ProperTerms *)
-Definition OT_leq {A} : relation (ProperTerm A) :=
-  fun x y => ot_R A (get_proper_term x) (get_proper_term y).
-
-(* Equivalence on ProperTerms *)
-Definition OT_equiv {A:OType} : relation (ProperTerm A) :=
-  fun x y => OT_leq x y /\ OT_leq y x.
+(* Build an OTerm for a function, with weaken_context already pre-applied *)
+Definition pfun_lambda' {ctx} {A} {B}
+        (f: (forall {ctx'} `{ext: OTCtxExtends (OTpair ctx A) ctx'},
+                OTermInCtx ctx' A) -> OTermInCtx (OTpair ctx A) B) :
+  OTermInCtx ctx (OTarrow A B) :=
+  mkOTermInCtx
+    (pfun_curry
+       (elimOTermInCtx (f (fun {ctx' ext} =>
+                             weaken_context (top_var_in_context ctx A))))).
 
 
-(***
- *** Builders for Proper Terms using OTPairInCtx
- ***)
-
-(* Helper to build a ProperTerm for a function *)
-Program Definition proper_fun {ctx} {A} {B}
-        (f: (forall {ctx'} `{ext: OTCtxExtends (A::ctx) ctx'},
-               OTPairInCtx ctx' A) ->
-            OTPairInCtx (A::ctx) B) :
-  OTPairInCtx ctx (OTArrow A B) :=
-  let (y1,y2,pf_y) :=
-      f (fun {ctx'} {ext} => weaken_context (ext:=ext) (top_var_in_context ctx A))
-  in
-  mkOTPairInCtx _ _ (fun ctx_elem x => y1 (x,ctx_elem))
-           (fun ctx_elem x => y2 (x,ctx_elem)) _.
-Next Obligation.
-  destruct pf_y as [ pf1 pf2 pf3 ].
-  repeat split; intros; [ apply pf1 | apply pf2 | apply pf3 ];
-  apply ctx_elem_lt_cons; assumption.
-Qed.
-
-(* Helper to implicitly add the arguments for a ProperTerm variable *)
-Definition proper_var {ctx} {A}
-           (var: (forall ctx' (ext: OTCtxExtends (A::ctx) ctx'),
-                    OTPairInCtx ctx' A))
-           {ctx'} {ext: OTCtxExtends (A::ctx) ctx'} :
-  OTPairInCtx ctx' A :=
-  var ctx' ext.
-
-
-(* Helper to build a ProperTerm for an application *)
-Program Definition proper_apply {ctx} {A} {B}
-        (f: OTPairInCtx ctx (OTArrow A B))
-        (x: OTPairInCtx ctx A) : OTPairInCtx ctx B :=
-  map2_OTPairInCtx (A:=OTArrow A B) (fun g y => g y) _ f x.
-Next Obligation.
-  intros f1 f2 pf_f; destruct pf_f as [ pf_f1 pf_f2 pf_f3 ];
-  intros x1 x2 pf_x; destruct pf_x as [ pf_x1 pf_x2 pf_x3 ];
-  repeat split;
-  first [ apply pf_f1 | apply pf_f2 | apply pf_f3 ];
-  repeat split; assumption.
-Qed.
-
-(* Helper to build a ProperProp for the leq relation of an OType *)
-Program Definition proper_leq {ctx} {A}
-        (x: OTPairInCtx ctx (OTFlip A))
-        (y: OTPairInCtx ctx A) : OTPairInCtx ctx OTProp :=
-
-  map2_OTPairInCtx (A:=OTFlip A) (C:=OTProp) (fun x y => ot_R A x y) _ x y.
-Next Obligation.
-  repeat (intro; intros); destruct H; destruct H0.
-  split; intro; try assumption.
-  apply (semitransitivity (SemiTransitive:=A) _ x0); try assumption.
-  apply (semitransitivity (SemiTransitive:=A) _ x1); try assumption.
-Qed.
-
-(* Helper to build a ProperTerm for a pair *)
-Program Definition proper_pair {ctx} {A} {B}
-           (x: OTPairInCtx ctx A) (y: OTPairInCtx ctx B) :
-  OTPairInCtx ctx (OTProd A B) :=
-  map2_OTPairInCtx (C:=OTProd A B) (fun x y => (x,y)) _ x y.
-Next Obligation.
-repeat (intro; intros); destruct H; destruct H0.
-unfold fst, snd; repeat split; assumption.
-Qed.
-
-(* Helper to build a ProperTerm for a first projection *)
-Program Definition proper_proj1 {ctx} {A} {B}
-           (x: OTPairInCtx ctx (OTProd A B)) : OTPairInCtx ctx A :=
-  map_OTPairInCtx (A:=OTProd A B) (fun p => fst p) _ x.
-Next Obligation.
-  intros p1 p2; destruct p1; destruct p2; unfold fst;
-  intro pf_p; destruct pf_p.
-  destruct H; destruct H0; destruct H1.
-  repeat split; assumption.
-Qed.
-
-(* Helper to build a ProperTerm for a second projection *)
-Program Definition proper_proj2 {ctx} {A} {B}
-           (x: OTPairInCtx ctx (OTProd A B)) : OTPairInCtx ctx B :=
-  map_OTPairInCtx (A:=OTProd A B) (fun p => snd p) _ x.
-Next Obligation.
-  intros p1 p2; destruct p1; destruct p2; unfold snd;
-  intro pf_p; destruct pf_p.
-  destruct H; destruct H0; destruct H1.
-  repeat split; assumption.
-Qed.
-
-(* Helper to build a ProperTerm for the inl constructor *)
-Program Definition proper_inl {ctx} {A} {B}
-           (x: OTPairInCtx ctx A) : OTPairInCtx ctx (OTSum A B) :=
-  map_OTPairInCtx (B:=OTSum A B) (fun y => inl y) _ x.
-Next Obligation.
-  intros x1 x2 pf_x; destruct pf_x; split; assumption.
-Qed.
-
-(* Helper to build a ProperTerm for the inr constructor *)
-Program Definition proper_inr {ctx} {A} {B}
-           (x: OTPairInCtx ctx B) : OTPairInCtx ctx (OTSum A B) :=
-  map_OTPairInCtx (B:=OTSum A B) (fun y => inr y) _ x.
-Next Obligation.
-  intros x1 x2 pf_x; destruct pf_x; split; assumption.
-Qed.
-
-(* Helper to build a ProperTerm for sum elimination *)
-Program Definition proper_sum_elim {ctx} {A} {B} {C}
-           (x: OTPairInCtx ctx (OTSum A B))
-           (f1: OTPairInCtx ctx (OTArrow A C))
-           (f2: OTPairInCtx ctx (OTArrow B C))
-: OTPairInCtx ctx C :=
-  map3_OTPairInCtx (A:=OTSum A B) (B:=OTArrow A C) (C:=OTArrow B C)
-                   (fun y g1 g2 => match y with
-                                     | inl y1 => g1 y1
-                                     | inr y2 => g2 y2
-                                   end) _ x f1 f2.
-Next Obligation.
-  intros sum1 sum2; destruct sum1; destruct sum2;
-  intros H g1 g2 pf_g h1 h2 pf_h; destruct H;
-  destruct pf_g as [ pf_g1 pf_g2 pf_g3 ];
-  destruct pf_h as [ pf_h1 pf_h2 pf_h3 ];
-  repeat split;
-  first [ apply pf_g1 | apply pf_g2 | apply pf_g3
-          | apply pf_h1 | apply pf_h2 | apply pf_h3
-          | elimtype False; assumption ];
-  repeat split; assumption.
-Qed.
-
-(* Existentials for OTProp *)
-Program Definition proper_exists {ctx} {A}
-        (f: OTPairInCtx ctx (OTArrow A OTProp)) : OTPairInCtx ctx OTProp :=
-  map_OTPairInCtx (A:= OTArrow A OTProp) (B:=OTProp)
-                  (fun f => exists x, ot_R A x x /\ f x) _ f.
-Next Obligation.
-  intros f1 f2 pf_f; destruct pf_f as [ pf_f1 pf_f2 pf_f3 ].
-  split; intro; try assumption.
-  destruct H as [ x H ]; destruct H.
-  exists x; split; [ assumption | ].
-  unfold Basics.impl in pf_f3; apply (pf_f3 x).
-  split; assumption. assumption.
-Qed.
-
-(* Conjunction for OTProp *)
-Program Definition proper_and {ctx} (P: OTPairInCtx ctx OTProp)
-        (Q: OTPairInCtx ctx OTProp) : OTPairInCtx ctx OTProp :=
-  map2_OTPairInCtx (A:=OTProp) (B:=OTProp) (C:=OTProp)
-                   (fun P Q => P /\ Q) _ P Q.
-Next Obligation.
-  unfold Basics.impl.
-  intros P1 P2 P_pf Q1 Q2 Q_pf.
-  destruct P_pf as [ P_pf1 P_pf2 P_pf3 ].
-  destruct Q_pf as [ Q_pf1 Q_pf2 Q_pf3 ].
-  split; intro; try assumption.
-  destruct H; split; [ apply P_pf3 | apply Q_pf3 ]; assumption.
-Qed.
+Definition ex1 : OTermInCtx OTunit (OTarrow OTnat OTnat) :=
+  pfun_lambda'
+    (fun (x : forall {ctx' ext}, _) => x).
 
 
 (***
